Construct convertAllowable
Signed-off-by: zeramorphic <zeramorphic@proton.me>

ConNF/Counting/SpecSame.lean
@@ -148,6 +148,149 @@ theorem convertCondition_eq_convertLitter (A : ExtendedIndex β) (L : Litter)
     ⟨⟨A, inr (convertLitter hσS hσT hT A L h).toNearLitter⟩, (convertLitter_mem hσS hσT hT A L h)⟩ :=
   (convertCondition_litter hσS hσT hT A L h).choose_spec.2
 
+@[simp]
+theorem convertAtom_convertAtom (A : ExtendedIndex β) (a : Atom) (h : ⟨A, inl a⟩ ∈ S) :
+    convertAtom hσT hσS hT hS A (convertAtom hσS hσT hS hT A a h)
+      (convertAtom_mem hσS hσT hS hT A a h) = a := by
+  have := convertCondition_convertCondition hσS hσT ⟨⟨A, inl a⟩, h⟩
+  rw [convertCondition_eq_convertAtom, convertCondition_eq_convertAtom] at this
+  simp only [Subtype.mk.injEq, SupportCondition.mk.injEq, inl.injEq, true_and] at this
+  exact this
+
+@[simp]
+theorem convertLitter_convertLitter (A : ExtendedIndex β) (L : Litter)
+    (h : ⟨A, inr L.toNearLitter⟩ ∈ S) :
+    convertLitter hσT hσS hS A (convertLitter hσS hσT hT A L h)
+      (convertLitter_mem hσS hσT hT A L h) = L := by
+  have := convertCondition_convertCondition hσS hσT ⟨⟨A, inr L.toNearLitter⟩, h⟩
+  rw [convertCondition_eq_convertLitter, convertCondition_eq_convertLitter] at this
+  simp only [Subtype.mk.injEq, SupportCondition.mk.injEq, inr.injEq, true_and,
+    Litter.toNearLitter_injective.eq_iff] at this
+  exact this
+
+theorem convertAtom_injective {A : ExtendedIndex β} {a b : Atom}
+    (ha : ⟨A, inl a⟩ ∈ S) (hb : ⟨A, inl b⟩ ∈ S)
+    (h : convertAtom hσS hσT hS hT A a ha = convertAtom hσS hσT hS hT A b hb) :
+    a = b := by
+  have := convertAtom_convertAtom hσS hσT hS hT A a ha
+  simp_rw [h, convertAtom_convertAtom] at this
+  exact this.symm
+
+theorem convertLitter_injective {A : ExtendedIndex β} {L₁ L₂ : Litter}
+    (h₁ : ⟨A, inr L₁.toNearLitter⟩ ∈ S) (h₂ : ⟨A, inr L₂.toNearLitter⟩ ∈ S)
+    (h : convertLitter hσS hσT hT A L₁ h₁ = convertLitter hσS hσT hT A L₂ h₂) :
+    L₁ = L₂ := by
+  have := convertLitter_convertLitter hσS hσT hS hT A L₁ h₁
+  simp_rw [h, convertLitter_convertLitter] at this
+  exact this.symm
+
+@[simp]
+theorem typein_convertAtom (A : ExtendedIndex β) (a : Atom) (h : ⟨A, inl a⟩ ∈ S) :
+    typein T.r ⟨⟨A, inl (convertAtom hσS hσT hS hT A a h)⟩, convertAtom_mem hσS hσT hS hT A a h⟩ =
+    typein S.r ⟨⟨A, inl a⟩, h⟩ :=
+  by rw [← convertCondition_eq_convertAtom, typein_convertCondition]
+
+@[simp]
+theorem typein_convertLitter (A : ExtendedIndex β) (L : Litter) (h : ⟨A, inr L.toNearLitter⟩ ∈ S) :
+    typein T.r ⟨⟨A, inr (convertLitter hσS hσT hT A L h).toNearLitter⟩,
+      convertLitter_mem hσS hσT hT A L h⟩ =
+    typein S.r ⟨⟨A, inr L.toNearLitter⟩, h⟩ :=
+  by rw [← convertCondition_eq_convertLitter, typein_convertCondition]
+
+noncomputable def convert : StructAction β :=
+  fun A => {
+    atomMap := fun a => ⟨_, fun h => convertAtom hσS hσT hS hT A a h⟩
+    litterMap := fun L => ⟨_, fun h => (convertLitter hσS hσT hT A L h).toNearLitter⟩
+    atomMap_dom_small := by
+      refine S.small.preimage ?_
+      intros _ _ h
+      simp only [SupportCondition.mk.injEq, inl.injEq, true_and] at h
+      exact h
+    litterMap_dom_small := by
+      refine S.small.preimage ?_
+      intros _ _ h
+      simp only [SupportCondition.mk.injEq, inr.injEq, true_and,
+        Litter.toNearLitter_injective.eq_iff] at h
+      exact h
+  }
+
+@[simp]
+theorem convert_atomMap {A : ExtendedIndex β} {a : Atom}
+    {h : (⟨A, inl a⟩ : SupportCondition β) ∈ S} :
+    ((convert hσS hσT hS hT A).atomMap a).get h = convertAtom hσS hσT hS hT A a h :=
+  rfl
+
+@[simp]
+theorem convert_litterMap {A : ExtendedIndex β} {L : Litter}
+    {h : (⟨A, inr L.toNearLitter⟩ : SupportCondition β) ∈ S} :
+    ((convert hσS hσT hS hT A).litterMap L).get h = (convertLitter hσS hσT hT A L h).toNearLitter :=
+  rfl
+
+@[simp]
+theorem _root_.ConNF.mem_toNearLitter {a : Atom} {L : Litter} :
+    a ∈ L.toNearLitter ↔ a.1 = L :=
+  Iff.rfl
+
+@[simp]
+theorem convertAtom_fst {A : ExtendedIndex β} {a : Atom}
+    (h : (⟨A, inl a⟩ : SupportCondition β) ∈ S) :
+    (convertAtom hσS hσT hS hT A a h).1 =
+    convertLitter hσS hσT hT A a.1 (hS.fst_toNearLitter_mem h) := by
+  have hσ₁ := hσS.atom_spec A a a.1.toNearLitter h (hS.fst_toNearLitter_mem h) rfl
+  have hσ₂ := hσT.atom_spec A (convertAtom hσS hσT hS hT A a h)
+    (convertAtom hσS hσT hS hT A a h).1.toNearLitter (convertAtom_mem hσS hσT hS hT A a h)
+    (hT.fst_toNearLitter_mem (convertAtom_mem hσS hσT hS hT A a h)) rfl
+  rw [← convertCondition_eq_convertAtom] at hσ₂
+  simp only [OrdSupport.coe_sort_coe, typein_convertCondition, hσ₁, SpecCondition.atom.injEq,
+    true_and] at hσ₂
+  have := congr_arg (typein T.r)
+    (convertCondition_eq_convertLitter hσS hσT hT A a.1 (hS.fst_toNearLitter_mem h))
+  simp only [OrdSupport.coe_sort_coe, typein_convertCondition, hσ₂, typein_inj, Subtype.mk.injEq,
+    SupportCondition.mk.injEq, inr.injEq, true_and, Litter.toNearLitter_injective.eq_iff] at this
+  exact this
+
+theorem convert_lawful : StructAction.Lawful (convert hσS hσT hS hT) :=
+  fun A => {
+    atomMap_injective := fun a b ha hb h => convertAtom_injective hσS hσT hS hT ha hb h
+    litterMap_injective := by
+      intro L₁ L₂ h₁ h₂ h
+      refine convertLitter_injective hσS hσT hS hT h₁ h₂ ?_
+      obtain ⟨a, ha₁, ha₂⟩ := h
+      exact eq_of_mem_litterSet_of_mem_litterSet ha₁ ha₂
+    atom_mem := by
+      intro a ha L hL
+      simp only [convert_atomMap, convert_litterMap, mem_toNearLitter, convertAtom_fst]
+      constructor
+      · rintro rfl
+        rfl
+      · exact convertLitter_injective hσS hσT hS hT (hS.fst_toNearLitter_mem ha) hL
+  }
+
+theorem convert_mapFlexible : StructAction.MapFlexible (convert hσS hσT hS hT) := by
+  intro A L hL₁ hL₂
+  have hLS := hσS.flexible_spec A L.toNearLitter hL₁ hL₂
+  obtain (hL | ⟨⟨hL⟩⟩ | ⟨⟨hL⟩⟩) := flexible_cases' β A (convertLitter hσS hσT hT A L hL₁)
+  · exact hL
+  · exfalso
+    obtain ⟨_, hLT⟩ := hσT.inflexibleBot_spec A _ (convertLitter_mem hσS hσT hT A L hL₁) hL
+    simp only [OrdSupport.coe_sort_coe, typein_convertLitter, hLS, Litter.toNearLitter_fst] at hLT
+  · exfalso
+    obtain ⟨χ, _, _, hLT⟩ := hσT.inflexibleCoe_spec A _ (convertLitter_mem hσS hσT hT A L hL₁) hL
+    simp only [OrdSupport.coe_sort_coe, typein_convertLitter, hLS, Litter.toNearLitter_fst] at hLT
+
+noncomputable def convertAllowable : Allowable β :=
+  (StructApprox.freedom_of_action β
+    (StructAction.rc (convert hσS hσT hS hT) (convert_lawful hσS hσT hS hT))
+    (StructAction.rc_free _ _ (convert_mapFlexible hσS hσT hS hT))).choose
+
+theorem convertAllowable_spec :
+    (StructAction.rc (convert hσS hσT hS hT)
+      (convert_lawful hσS hσT hS hT)).ExactlyApproximates
+    (Allowable.toStructPerm (convertAllowable hσS hσT hS hT)) :=
+  (StructApprox.freedom_of_action β
+    (StructAction.rc (convert hσS hσT hS hT) (convert_lawful hσS hσT hS hT))
+    (StructAction.rc_free _ _ (convert_mapFlexible hσS hσT hS hT))).choose_spec
+
 end Spec
 
 end ConNF
